Readme.md
@@ -2,10 +2,13 @@ A simple verified compiler, from the (simple typed, call-by-value) lambda calcul
 
 Goals:
 
-Complete missing steps (currently in Assemble and disassemble)
+Complete missing steps (currently in typechecking)
 Figure out use for other direction of correctness proofs?
 Modularize code with classes
-Remove tags
+Remove runtime tags
 User types for printing
 Add Parser?
 Add pairs, sums, unit, void, nats, primrec? sructured types?
+Make printing part of the code
+Make initializagtion part of the code
+Use aegbraic compiler
